Fixed the overflow-flag semantics for ADD, ADC, SUB, NEG, CMP.
Fixed the carry and overflow flag semantics for IMUL.

x86model/Model/SemTests.v
@@ -20,6 +20,7 @@ Arguments Word.mone {_}.
 
 Section InitState.
 Variable eax ebx ecx : int32.
+Variable cf: int1.
 
 Definition empty_mem : AddrMap.t int8 := (Word.zero, PTree.empty _).
 Definition empty_seg : fmap segment_register int32 := (fun seg => Word.zero).
@@ -84,6 +85,40 @@ Definition no_prefix : prefix := mkPrefix None None false false.
 Definition run (i:instr) :=
   RTL_step_list (instr_to_rtl no_prefix i) init_rtl_state.
 
+Definition flags_cf : fmap flag int1 := 
+  fun f => if flag_eq_dec f CF then cf else Word.zero.
+
+Definition init_machine_cf : core_state. 
+  refine {|
+    gp_regs := init_reg;
+    seg_regs_starts := empty_seg;
+    seg_regs_limits := (fun seg_reg => Word.mone);
+    flags_reg := flags_cf;
+    control_regs := (fun c => Word.zero);
+    debug_regs :=  (fun d => Word.zero);
+    pc_reg := init_pc
+  |}.
+Defined.
+
+Definition init_full_machine_cf : mach_state.
+  refine {|
+   core := init_machine_cf;
+   fpu := empty_fpu_machine
+  |}.
+Defined.
+
+Definition init_rtl_state_cf : rtl_state.
+  refine {|
+    rtl_oracle := empty_oracle;
+    rtl_env := empty_env;
+    rtl_mach_state := init_full_machine_cf;
+    rtl_memory := empty_mem
+  |}.
+Defined.
+
+Definition runWithCF (i:instr) :=
+  RTL_step_list (instr_to_rtl no_prefix i) init_rtl_state_cf.
+
 Definition gpr (s:@RTL_ans unit * rtl_state) :=
   gp_regs (core (rtl_mach_state (snd s))).
 
@@ -93,6 +128,7 @@ Definition flag (s:@RTL_ans unit * rtl_state) :=
 End InitState.
 
 Module Test_XOR.
+
   Definition i:instr := XOR true (Reg_op EAX) (Reg_op EBX).
 
   (* Compute (instr_to_rtl no_prefix i). *)
@@ -100,29 +136,56 @@ Module Test_XOR.
 
   (* PF should be zero since (gpr (run one zero zero i) EAX) is 1,
      which has an odd number of bits *)
-  Example ex1: (flag (run one zero zero i) PF) = zero.
+  Goal (flag (run one zero zero i) PF) = zero.
   Proof. reflexivity. Qed.
 
 End Test_XOR.
 
 Module Test_Add.
-  Definition i:instr := ADD true (Reg_op EAX) (Reg_op EBX).
 
-  (* Compute (gpr  (run one mone zero i) EAX). *)
+  Definition i1:instr := ADD true (Reg_op EAX) (Reg_op EBX).
 
   (* ZF should be one, since (gpr  (run one mone zero i) EAX)
      returns zero *)
-  Example ex1: (flag (run one mone zero i) ZF) = one.
+  Goal (flag (run one mone zero i1) ZF) = one.
+  Proof. reflexivity. Qed.
+
+  Goal (flag (run one mone zero i1) OF) = zero.
+  Proof. reflexivity. Qed.
+
+  Goal (flag (run (repr 2147483648) (repr 2147483648) zero i1) OF) = one.
   Proof. reflexivity. Qed.
 
 End Test_Add.
 
 Module Test_Adc.
+
   Definition i:instr := 
     ADC true (Reg_op (EBX)) (Reg_op (ECX)).
 
-  Example ex1: (gpr (run zero (repr 2146959366) (repr 2148007937) i) EBX)
+  Goal (gpr (run zero (repr 2146959366) (repr 2148007937) i) EBX)
               = repr 7.
+  Proof. reflexivity. Qed.
+
+  Goal (flag (run zero (repr 2146959366) (repr 2148007937) i) OF) = zero.
+  Proof. reflexivity. Qed.
+
+  Goal (gpr (run zero (repr 2146959366) (repr 2148007937) i) EBX) = repr 7.
+  Proof. reflexivity. Qed.
+
+  Goal (flag (runWithCF zero (repr 7) (repr 2148007937) one i) OF) = zero.
+  Proof. reflexivity. Qed.
+
+  Goal (flag (runWithCF zero (repr 67373084) (repr 3756307471) one i) OF) = zero.
+  Proof. reflexivity. Qed.
+
+  Goal (flag (runWithCF zero (repr 2036070270) (repr 111413377) one i) OF) = one.
+  Proof. reflexivity. Qed.
+
+  Goal (flag (runWithCF zero zero zero one i) OF) = zero.
+  Proof. reflexivity. Qed.
+
+  Goal (flag (runWithCF zero (repr 4294967295) (repr 4294967295) one i) OF) = zero.
   Proof. reflexivity. Qed.
 
 End Test_Adc.
@@ -130,28 +193,28 @@ End Test_Adc.
 Module Test_Sbb.
   Definition i:instr := SBB true (Reg_op (EBX)) (Reg_op (ECX)).
 
-  Example ex1: (gpr (run zero (repr 3221249032) (repr 3221249032) i) EBX)
+  Goal (gpr (run zero (repr 3221249032) (repr 3221249032) i) EBX)
               = repr 0.
   Proof. reflexivity. Qed.
 
-  Example ex2: (flag (run zero (repr 3221249032) (repr 3221249032) i) ZF)
+  Goal (flag (run zero (repr 3221249032) (repr 3221249032) i) ZF)
               = repr 1.
   Proof. reflexivity. Qed.
 
-  Example ex3: (flag (run zero (repr 3221249032) (repr 3221249032) i) PF)
+  Goal (flag (run zero (repr 3221249032) (repr 3221249032) i) PF)
               = repr 1.
   Proof. reflexivity. Qed.
 
-  Example ex4: (flag (run zero (repr 3221249032) (repr 3221249032) i) SF)
+  Goal (flag (run zero (repr 3221249032) (repr 3221249032) i) SF)
               = repr 0.
   Proof. reflexivity. Qed.
 
-  Example ex5: (flag (run zero (repr 3221249032) (repr 3221249032) i) CF)
+  Goal (flag (run zero (repr 3221249032) (repr 3221249032) i) CF)
               = repr 0.
   Proof. reflexivity. Qed.
 
   (* this fails for now *)
-  (* Example ex6: (flag (run zero (repr 2147483712) (repr 2147483648) i) OF) *)
+  (* Goal (flag (run zero (repr 2147483712) (repr 2147483648) i) OF) *)
   (*             = repr 0. *)
   (* Proof. reflexivity. Qed. *)
 
@@ -160,11 +223,11 @@ End Test_Sbb.
 Module Test_Xadd.
   Definition i:instr := XADD true (Reg_op (EBX)) (Reg_op (ECX)).
 
-  Example ex1: (flag (run zero (repr 1608135424) (repr 2759947009) i) OF)
+  Goal (flag (run zero (repr 1608135424) (repr 2759947009) i) OF)
               = repr 0.
   Proof. reflexivity. Qed.
 
-  Example ex2: intval 31 (gpr (run zero (repr 1608135424) (repr 2759947009) i) EBX)
+  Goal intval 31 (gpr (run zero (repr 1608135424) (repr 2759947009) i) EBX)
               = intval 31 (repr 73115137).
   Proof. reflexivity. Qed.
 
@@ -173,32 +236,62 @@ End Test_Xadd.
 Module Test_Mul.
   Definition i:instr := MUL true (Reg_op (EBX)).
 
-  Example ex1: (gpr (run (repr 2233468006) (repr 1546826500) zero i) EDX)
-               =  (repr 804380396).
+  Goal gpr (run (repr 2233468006) (repr 1546826500) zero i) EDX
+       =  (repr 804380396).
+  Proof. reflexivity. Qed.
+
+  Goal flag (run (repr 1242038273) (repr 3052929025) zero i) CF = one.
   Proof. reflexivity. Qed.
 
 End Test_Mul.
 
 Module Test_Imul.
-  Definition i:instr := IMUL true (Reg_op (EBX)) (None) (None).
+  Definition i:instr := IMUL true (Reg_op EBX) None None.
 
-  Example ex1: (gpr (run (repr 633430437) (repr 2147483231) zero i) EDX)
+  Goal (gpr (run (repr 633430437) (repr 2147483231) zero i) EDX)
                =  (repr 316715156).
   Proof. reflexivity. Qed.
 
+  Goal (flag (run (repr 633430437) (repr 2147483231) zero i) CF) = one.
+  Proof. reflexivity. Qed.
+
+  Goal flag (run (repr 4294967261) (repr 109051904) zero i) CF = one.
+  Proof. reflexivity. Qed.
+
   (* SF is undefined according to manual *)
-  (* Example ex2: (flag (run (repr 633430437) (repr 2147483231) zero i) SF) *)
+  (* Goal (flag (run (repr 633430437) (repr 2147483231) zero i) SF) *)
   (*              =  (repr 1). *)
   (* Proof. reflexivity. Qed. *)
 
 
 End Test_Imul.
 
-Module SubOverflow.
+Module Test_Sub.
+
   Definition i:instr := SUB true (Reg_op EAX) (Reg_op EBX).
 
-  (* the overflow flags is not set, even though the result overflowed to -3 *)
-  Compute (gpr  (run (repr 2147483645) (repr 2147483648) zero i) EAX).
-  Compute (flag (run (repr 2147483645) (repr 2147483648) zero i) OF).
-End SubOverflow.
+  Goal (flag (run (repr 2147483645) (repr 2147483648) zero i) OF = one).
+  Proof. reflexivity. Qed.
 
+  Goal (flag (run (repr 2684354560) (repr 2147483648) zero i) OF = zero).
+  Proof. reflexivity. Qed.
+
+End Test_Sub.
+
+Module Test_Cmp.
+
+  Definition i:instr := CMP true (Reg_op EBX) (Reg_op ECX).
+
+  Goal (flag (run zero zero (repr 2147483648) i) OF = one).
+  Proof. reflexivity. Qed.
+
+End Test_Cmp.
+
+Module Test_Neg.
+
+  Definition i:instr := NEG true (Reg_op EBX).
+
+  Goal flag (run zero (repr 2147483648) zero i) OF = one.
+  Proof. reflexivity. Qed.
+
+End Test_Neg.
